queue: some renaming for clarity

misc/queue-basic-known.bpl
@@ -109,12 +109,12 @@ type Key;
 var {:layer 0, 1} next: [Ref]Ref;
 var {:layer 0, 1} data: [Ref]Key;
 
-var {:linear "FP"} {:layer 0, 1} queueFP: [Ref]bool;
-var {:linear "FP"} {:layer 0, 1} UsedFP: [Ref]bool;
+var {:linear "FP"} {:layer 0, 1} queueFP: [Ref]bool;  // TODO make layer 1,1 and intro actions to modify?
+var {:linear "FP"} {:layer 0, 1} usedFP: [Ref]bool;
 
 var {:layer 0, 1} head: Ref;
 var {:layer 0, 1} tail: Ref;
-var {:layer 0, 1} start: Ref; // The first head. To define UsedFP
+var {:layer 0, 1} start: Ref; // The first head. To define usedFP
 
 
 // Abstract state
@@ -124,7 +124,7 @@ var {:layer 1,2} absTail: int;
 var {:layer 1,2} absRefs: [int]Ref;  // connection between abstract and concrete
 
 
-function {:inline} Inv(queueFP: [Ref]bool, UsedFP: [Ref]bool, start: Ref,
+function {:inline} Inv(queueFP: [Ref]bool, usedFP: [Ref]bool, start: Ref,
     head: Ref, tail: Ref, next: [Ref]Ref, data: [Ref]Key,
     absArray: [int]Key, absRefs: [int]Ref, absHead: int, absTail: int) : (bool)
 {
@@ -134,10 +134,10 @@ function {:inline} Inv(queueFP: [Ref]bool, UsedFP: [Ref]bool, start: Ref,
     known(x) ==> (queueFP[x] <==> (Btwn(next, head, x, null) && x != null)))
   // Tail is on that list
   && Btwn(next, head, tail, null) && tail != null
-  // There is also a list from start to head
+  // There is also a list from start to head // TODO try just lseg(c, head)
   && Btwn(next, start, start, head)
-  && (forall x: Ref :: {UsedFP[x]}{Btwn(next, start, x, head)}
-    known(x) ==> (UsedFP[x] <==> (Btwn(next, start, x, head) && x != head)))
+  && (forall x: Ref :: {usedFP[x]}{Btwn(next, start, x, head)}
+    known(x) ==> (usedFP[x] <==> (Btwn(next, start, x, head) && x != head)))
   // Terms needed for axiom triggers
   && known(start) && known(head) && known(tail) && known(null) && knownF(next)
   // Properties of abstract state
@@ -155,17 +155,17 @@ function {:inline} Inv(queueFP: [Ref]bool, UsedFP: [Ref]bool, start: Ref,
 
 // ---------- Primitives for manipulating global state
 
-procedure {:atomic} {:layer 1} AtomicReadhead() returns (x: Ref)
+procedure {:atomic} {:layer 1} readHead_atomic() returns (x: Ref)
 { x := head; }
 
-procedure {:yields} {:layer 0} {:refines "AtomicReadhead"} Readhead() returns (x: Ref);
+procedure {:yields} {:layer 0} {:refines "readHead_atomic"} readHead() returns (x: Ref);
 
-procedure {:atomic} {:layer 1} AtomicReadtail() returns (x: Ref)
+procedure {:atomic} {:layer 1} readTail_atomic() returns (x: Ref)
 { x := tail; }
 
-procedure {:yields} {:layer 0} {:refines "AtomicReadtail"} Readtail() returns (x: Ref);
+procedure {:yields} {:layer 0} {:refines "readTail_atomic"} readTail() returns (x: Ref);
 
-procedure {:atomic} {:layer 1} AtomicCasTail(ole: Ref, new: Ref) returns (b: bool)
+procedure {:atomic} {:layer 1} casTail_atomic(ole: Ref, new: Ref) returns (b: bool)
   modifies tail;
 {
   if (tail == ole) {
@@ -176,84 +176,83 @@ procedure {:atomic} {:layer 1} AtomicCasTail(ole: Ref, new: Ref) returns (b: boo
   }
 }
 
-procedure {:yields} {:layer 0} {:refines "AtomicCasTail"}
-  CasTail(ole: Ref, new: Ref) returns (b: bool);
+procedure {:yields} {:layer 0} {:refines "casTail_atomic"}
+  casTail(ole: Ref, new: Ref) returns (b: bool);
 
-procedure {:atomic} {:layer 1} readNext_spec(i:Ref) returns (x: Ref)
+procedure {:atomic} {:layer 1} readNext_atomic(x: Ref) returns (y: Ref)
 {
-  assert queueFP[i] || UsedFP[i];
-  x := next[i];
-  assume known(x);
+  assert queueFP[x] || usedFP[x];
+  y := next[x];
+  assume known(y);
 }
 
-procedure {:yields} {:layer 0} {:refines "readNext_spec"} readNext(i:Ref) returns (x: Ref);
+procedure {:yields} {:layer 0} {:refines "readNext_atomic"} readNext(x: Ref) returns (y: Ref);
 
-procedure {:atomic} {:layer 1} readData_spec(x: Ref) returns (v: Key)
+procedure {:atomic} {:layer 1} readData_atomic(x: Ref) returns (k: Key)
 {
-  assert queueFP[x] || UsedFP[x];
-  v := data[x];
+  assert queueFP[x] || usedFP[x];
+  k := data[x];
 }
 
-procedure {:yields} {:layer 0} {:refines "readData_spec"} readData(x: Ref) returns (v: Key);
+procedure {:yields} {:layer 0} {:refines "readData_atomic"} readData(x: Ref) returns (k: Key);
 
-procedure {:atomic} {:layer 1} AtomicStore({:linear "FP"} FP:[Ref]bool,
-    i:Ref, x: Ref)
+procedure {:atomic} {:layer 1} writeNext_atomic(x: Ref, y: Ref, {:linear "FP"} FP:[Ref]bool)
   modifies next;
 {
-  assert FP[i];
-  next := next[i := x];
+  assert FP[x];
+  next := next[x := y];
   assume knownF(next);
 }
 
-procedure {:yields} {:layer 0} {:refines "AtomicStore"}
-  Store({:linear "FP"} FP:[Ref]bool, i:Ref, x: Ref);
+procedure {:yields} {:layer 0} {:refines "writeNext_atomic"}
+  writeNext(x: Ref, y: Ref, {:linear "FP"} FP:[Ref]bool);
 
-procedure {:atomic} {:layer 1} AtomicTransferToqueue(t: Ref, oldVal: Ref,
-    newVal: Ref, {:linear_in "FP"} l_in:[Ref]bool)
-  returns (r: bool, {:linear "FP"} l_out:[Ref]bool)
+procedure {:atomic} {:layer 1} casNextTransfer_atomic(x: Ref, oldVal: Ref,
+    newVal: Ref, {:linear_in "FP"} inFP:[Ref]bool)
+  returns (b: bool, {:linear "FP"} outFP:[Ref]bool)
   modifies next, queueFP;
 {
-  assert l_in[newVal];
-  if (next[t] == oldVal) {
-    next := next[t := newVal];
-    l_out := emptySet;
+  assert inFP[newVal];
+  if (next[x] == oldVal) {
+    next := next[x := newVal];
+    outFP := emptySet;
     queueFP := queueFP[newVal := true];
     assume knownF(next);
-    r := true;
+    b := true;
   } else {
-    l_out := l_in;
-    r := false;
+    outFP := inFP;
+    b := false;
   }
 }
 
-procedure {:yields} {:layer 0} {:refines "AtomicTransferToqueue"}
-  TransferToqueue(t: Ref, oldVal: Ref, newVal: Ref,
-                  {:linear_in "FP"} l_in:[Ref]bool)
-  returns (r: bool, {:linear "FP"} l_out:[Ref]bool);
+procedure {:yields} {:layer 0} {:refines "casNextTransfer_atomic"}
+  casNextTransfer(x: Ref, oldVal: Ref, newVal: Ref, {:linear_in "FP"} inFP:[Ref]bool)
+  returns (b: bool, {:linear "FP"} outFP:[Ref]bool);
 
-procedure {:atomic} {:layer 1} AtomicTransferFromqueue(oldVal: Ref, newVal: Ref) returns (r: bool)
-  modifies head, UsedFP, queueFP;
+procedure {:atomic} {:layer 1} casHeadTransfer_atomic(oldVal: Ref, newVal: Ref) returns (b: bool)
+  modifies head, usedFP, queueFP;
 {
   if (oldVal == head) {
     head := newVal;
-    UsedFP[oldVal] := true;
+    usedFP[oldVal] := true;
     queueFP := queueFP[oldVal := false];
-    r := true;
+    b := true;
   }
   else {
-    r := false;
+    b := false;
   }
 }
 
-procedure {:yields} {:layer 0} {:refines "AtomicTransferFromqueue"} TransferFromqueue(oldVal: Ref, newVal: Ref) returns (r: bool);
+procedure {:yields} {:layer 0} {:refines "casHeadTransfer_atomic"}
+  casHeadTransfer(oldVal: Ref, newVal: Ref) returns (b: bool);
 
 
 // ---------- Primitives for manipulating logical/abstract state
 
-procedure {:layer 1} {:inline 1} intro_writeAbs(v: Key, x: Ref)
+procedure {:layer 1} {:inline 1} intro_writeAbs(k: Key, x: Ref)
   modifies absArray, absRefs;
 {
-  absArray[absTail] := v;
+  absArray[absTail] := k;
   absRefs[absTail] := x;
 }
 
@@ -272,162 +271,163 @@ procedure {:layer 1} {:inline 1} intro_incrTail()
 
 // ---------- queue methods:
 
-procedure {:atomic} {:layer 2} atomic_pop() returns (v: Key)
+procedure {:atomic} {:layer 2} atomic_pop() returns (k: Key)
   modifies absHead;
 {
-  v := absArray[absHead];
+  k := absArray[absHead];
   absHead := absHead + 1;
 }
 
-procedure {:yields} {:layer 1} {:refines "atomic_pop"} pop() returns (v: Key)
-  requires {:layer 1} Inv(queueFP, UsedFP, start, head, tail, next, data, absArray, absRefs, absHead, absTail);
-  ensures {:layer 1} Inv(queueFP, UsedFP, start, head, tail, next, data, absArray, absRefs, absHead, absTail);
+procedure {:yields} {:layer 1} {:refines "atomic_pop"} pop() returns (k: Key)
+  requires {:layer 1} Inv(queueFP, usedFP, start, head, tail, next, data, absArray, absRefs, absHead, absTail);
+  ensures {:layer 1} Inv(queueFP, usedFP, start, head, tail, next, data, absArray, absRefs, absHead, absTail);
 {
   var g: bool;
   var h, t, x: Ref;
 
   yield;
-  assert {:layer 1} Inv(queueFP, UsedFP, start, head, tail, next, data, absArray, absRefs, absHead, absTail);
+  assert {:layer 1} Inv(queueFP, usedFP, start, head, tail, next, data, absArray, absRefs, absHead, absTail);
   while (true)
-    invariant {:layer 1} Inv(queueFP, UsedFP, start, head, tail, next, data, absArray, absRefs, absHead, absTail);
+    invariant {:layer 1} Inv(queueFP, usedFP, start, head, tail, next, data, absArray, absRefs, absHead, absTail);
   {
-    call h := Readhead();
+    call h := readHead();
     yield;
-    assert {:layer 1} Inv(queueFP, UsedFP, start, head, tail, next, data, absArray, absRefs, absHead, absTail);
-    assert {:layer 1} h == head || UsedFP[h];
+    assert {:layer 1} Inv(queueFP, usedFP, start, head, tail, next, data, absArray, absRefs, absHead, absTail);
+    assert {:layer 1} h == head || usedFP[h];
 
-    call t := Readtail();
+    call t := readTail();
     yield;
-    assert {:layer 1} Inv(queueFP, UsedFP, start, head, tail, next, data, absArray, absRefs, absHead, absTail);
-    assert {:layer 1} h == head || UsedFP[h];
+    assert {:layer 1} Inv(queueFP, usedFP, start, head, tail, next, data, absArray, absRefs, absHead, absTail);
+    assert {:layer 1} h == head || usedFP[h];
     assert {:layer 1} (h == head && h != t ==> head != tail);
 
     if (h != t) {
       call x := readNext(h);
       yield;
-      assert {:layer 1} Inv(queueFP, UsedFP, start, head, tail, next, data, absArray, absRefs, absHead, absTail);
-      assert {:layer 1} h == head || UsedFP[h];
+      assert {:layer 1} Inv(queueFP, usedFP, start, head, tail, next, data, absArray, absRefs, absHead, absTail);
+      assert {:layer 1} h == head || usedFP[h];
       assert {:layer 1} (h == head && h != t ==> head != tail && x == next[head]);
 
-      call v := readData(h);
+      call k := readData(h);
       yield;
-      assert {:layer 1} Inv(queueFP, UsedFP, start, head, tail, next, data, absArray, absRefs, absHead, absTail);
-      assert {:layer 1} h == head || UsedFP[h];
+      assert {:layer 1} Inv(queueFP, usedFP, start, head, tail, next, data, absArray, absRefs, absHead, absTail);
+      assert {:layer 1} h == head || usedFP[h];
       assert {:layer 1} (h == head && h != t ==> head != tail && x == next[head]);
-      assert {:layer 1} data[h] == v;
+      assert {:layer 1} data[h] == k;
 
-      call g := TransferFromqueue(h, x);
+      call g := casHeadTransfer(h, x);
       if (g) {
         // Linearization point. Update abstract state:
         call intro_incrHead();
         break;
       }
-    }
+    }  // TODO return EMPTY?
     yield;
-    assert {:layer 1} Inv(queueFP, UsedFP, start, head, tail, next, data, absArray, absRefs, absHead, absTail);
+    assert {:layer 1} Inv(queueFP, usedFP, start, head, tail, next, data, absArray, absRefs, absHead, absTail);
   }
   yield;
-  assert {:expand} {:layer 1} Inv(queueFP, UsedFP, start, head, tail, next, data, absArray, absRefs, absHead, absTail);
+  assert {:expand} {:layer 1} Inv(queueFP, usedFP, start, head, tail, next, data, absArray, absRefs, absHead, absTail);
 }
 
 
-procedure {:atomic} {:layer 2} atomic_push(v: Key, x: Ref, {:linear_in "FP"} xFP: [Ref]bool)
+procedure {:atomic} {:layer 2} atomic_push(k: Key, x: Ref, {:linear_in "FP"} xFP: [Ref]bool)
   modifies absArray, absTail, absRefs;
 {
   absTail := absTail + 1;
   absRefs[absTail] := x;
-  absArray[absTail] := v;
+  absArray[absTail] := k;
 }
 
-procedure {:yields} {:layer 1} {:refines "atomic_push"} push(v: Key, x: Ref,
+procedure {:yields} {:layer 1} {:refines "atomic_push"} push(k: Key, x: Ref,
     {:linear_in "FP"} xFP: [Ref]bool)
-  requires {:layer 1} xFP[x] && next[x] == null && data[x] == v;  // TODO alloc x with v
+  requires {:layer 1} xFP[x] && next[x] == null && data[x] == k;  // TODO alloc x with k
   requires {:layer 1} !Btwn(next, head, x, null);  // TODO get from linearity
-  requires {:layer 1} Inv(queueFP, UsedFP, start, head, tail, next, data, absArray, absRefs, absHead, absTail);
-  ensures {:layer 1} Inv(queueFP, UsedFP, start, head, tail, next, data, absArray, absRefs, absHead, absTail);
+  requires {:layer 1} Inv(queueFP, usedFP, start, head, tail, next, data, absArray, absRefs, absHead, absTail);
+  ensures {:layer 1} Inv(queueFP, usedFP, start, head, tail, next, data, absArray, absRefs, absHead, absTail);
 {
   var t, tn: Ref;
   var g: bool;
   var {:linear "FP"} tFP: [Ref]bool;
 
   yield;
-  assert {:layer 1} Inv(queueFP, UsedFP, start, head, tail, next, data, absArray, absRefs, absHead, absTail);
+  assert {:layer 1} Inv(queueFP, usedFP, start, head, tail, next, data, absArray, absRefs, absHead, absTail);
   assert {:layer 1} !Btwn(next, head, x, null);
-  assert {:layer 1} xFP[x] && next[x] == null && data[x] == v;
+  assert {:layer 1} xFP[x] && next[x] == null && data[x] == k;
   tFP := xFP;
   while (true)
-    invariant {:layer 1} Inv(queueFP, UsedFP, start, head, tail, next, data, absArray, absRefs, absHead, absTail);
+    invariant {:layer 1} Inv(queueFP, usedFP, start, head, tail, next, data, absArray, absRefs, absHead, absTail);
     invariant {:layer 1} known(x) && !Btwn(next, head, x, null);
-    invariant {:layer 1} tFP == xFP && xFP[x] && next[x] == null && data[x] == v;
+    invariant {:layer 1} tFP == xFP && xFP[x] && next[x] == null && data[x] == k;
   {
-    call t := Readtail();
+    call t := readTail();
     yield;
-    assert {:layer 1} Inv(queueFP, UsedFP, start, head, tail, next, data, absArray, absRefs, absHead, absTail);
+    assert {:layer 1} Inv(queueFP, usedFP, start, head, tail, next, data, absArray, absRefs, absHead, absTail);
     assert {:layer 1} !Btwn(next, head, x, null);
-    assert {:layer 1} tFP == xFP && xFP[x] && next[x] == null && data[x] == v;
-    assert {:layer 1} t != null && (queueFP[t] || UsedFP[t]);
+    assert {:layer 1} tFP == xFP && xFP[x] && next[x] == null && data[x] == k;
+    assert {:layer 1} t != null && (queueFP[t] || usedFP[t]);
     assert {:layer 1} next[t] == null ==> queueFP[t];
 
     call tn := readNext(t);
     yield;
-    assert {:layer 1} Inv(queueFP, UsedFP, start, head, tail, next, data, absArray, absRefs, absHead, absTail);
+    assert {:layer 1} Inv(queueFP, usedFP, start, head, tail, next, data, absArray, absRefs, absHead, absTail);
     assert {:layer 1} !Btwn(next, head, x, null);
-    assert {:layer 1} tFP == xFP && xFP[x] && next[x] == null && data[x] == v;
-    assert {:layer 1} t != null && (queueFP[t] || UsedFP[t]);
+    assert {:layer 1} tFP == xFP && xFP[x] && next[x] == null && data[x] == k;
+    assert {:layer 1} t != null && (queueFP[t] || usedFP[t]);
     assert {:layer 1} next[t] == null ==> queueFP[t];
     assert {:layer 1} tn != null ==> tn == next[t];
 
     if (tn == null) {
-      call g, tFP := TransferToqueue(t, tn, x, tFP);
+      call g, tFP := casNextTransfer(t, tn, x, tFP);
       if (g) {
         // Linearization point. Update abstract state:
         call intro_incrTail();
-        call intro_writeAbs(v, x);
+        call intro_writeAbs(k, x);
         break;
       }
     } else {
-      call g := CasTail(t, tn);
+      call g := casTail(t, tn);
     }
     yield;
-    assert {:layer 1} Inv(queueFP, UsedFP, start, head, tail, next, data, absArray, absRefs, absHead, absTail);
+    assert {:layer 1} Inv(queueFP, usedFP, start, head, tail, next, data, absArray, absRefs, absHead, absTail);
     assert {:layer 1} !Btwn(next, head, x, null);
-    assert {:layer 1} tFP == xFP && xFP[x] && next[x] == null && data[x] == v;
+    assert {:layer 1} tFP == xFP && xFP[x] && next[x] == null && data[x] == k;
   }
   yield;
-  assert {:expand} {:layer 1} Inv(queueFP, UsedFP, start, head, tail, next, data, absArray, absRefs, absHead, absTail);
+  assert {:expand} {:layer 1} Inv(queueFP, usedFP, start, head, tail, next, data, absArray, absRefs, absHead, absTail);
 }
 
 
-procedure {:atomic} {:layer 2} atomic_size() returns (x: int)
+procedure {:atomic} {:layer 2} atomic_size() returns (s: int)
 {}
 
-procedure {:yields} {:layer 1} {:refines "atomic_size"} size() returns (x: int)
-  requires {:layer 1} Inv(queueFP, UsedFP, start, head, tail, next, data, absArray, absRefs, absHead, absTail);
-  ensures {:layer 1} Inv(queueFP, UsedFP, start, head, tail, next, data, absArray, absRefs, absHead, absTail);
+// Size invariant: s == indexOf[c] - old(absHead)
+procedure {:yields} {:layer 1} {:refines "atomic_size"} size() returns (s: int)
+  requires {:layer 1} Inv(queueFP, usedFP, start, head, tail, next, data, absArray, absRefs, absHead, absTail);
+  ensures {:layer 1} Inv(queueFP, usedFP, start, head, tail, next, data, absArray, absRefs, absHead, absTail);
 {
   var c: Ref;
 
   yield;
-  assert {:layer 1} Inv(queueFP, UsedFP, start, head, tail, next, data, absArray, absRefs, absHead, absTail);
+  assert {:layer 1} Inv(queueFP, usedFP, start, head, tail, next, data, absArray, absRefs, absHead, absTail);
 
-  x := 0;
-  call c := Readhead();
+  s := 0;
+  call c := readHead();
 
   yield;
-  assert {:layer 1} Inv(queueFP, UsedFP, start, head, tail, next, data, absArray, absRefs, absHead, absTail);
-  assert {:layer 1} (UsedFP[c] || queueFP[c]);
+  assert {:layer 1} Inv(queueFP, usedFP, start, head, tail, next, data, absArray, absRefs, absHead, absTail);
+  assert {:layer 1} (usedFP[c] || queueFP[c]);
 
   while (c != null)
-    invariant {:layer 1} Inv(queueFP, UsedFP, start, head, tail, next, data, absArray, absRefs, absHead, absTail);
-    invariant {:layer 1} known(c) && (UsedFP[c] || queueFP[c] || c == null);
+    invariant {:layer 1} Inv(queueFP, usedFP, start, head, tail, next, data, absArray, absRefs, absHead, absTail);
+    invariant {:layer 1} known(c) && (usedFP[c] || queueFP[c] || c == null);
   {
-    x := x + 1;
+    s := s + 1;
     call c := readNext(c);
     yield;
-    assert {:layer 1} Inv(queueFP, UsedFP, start, head, tail, next, data, absArray, absRefs, absHead, absTail);
-    assert {:layer 1} (UsedFP[c] || queueFP[c] || c == null);
+    assert {:layer 1} Inv(queueFP, usedFP, start, head, tail, next, data, absArray, absRefs, absHead, absTail);
+    assert {:layer 1} (usedFP[c] || queueFP[c] || c == null);
   }
   yield;
-  assert {:layer 1} Inv(queueFP, UsedFP, start, head, tail, next, data, absArray, absRefs, absHead, absTail);
+  assert {:layer 1} Inv(queueFP, usedFP, start, head, tail, next, data, absArray, absRefs, absHead, absTail);
   return;
 }
